Network_Security_Policy_Verification/Examples/Imaginary_Factory_Network.thy
@@ -1,0 +1,317 @@
+theory Imaginary_Factory_Network
+imports "../TopoS_Impl"
+begin
+
+
+(* scala_tool said:
+>>> eval
+
+Overview:
+[valid] BLPbasic: Privacy for employees
+[valid] BLPbasic: Secret corporate knowledge and intellectual propertiy
+[valid] BLPtrusted: Privacy for employees, exporting aggregated data
+[valid] CommunicationPartners: we subnet the whole fab!
+[valid] Dependability: blubb
+[valid] DomainHierarchy: Hierarchy of fab robots
+[valid] NonInterference: NonInterference of something
+[valid] SecurityGateway: Sensor Gateway
+[valid] Sink: Robots are sink
+[valid] Subnets: we subnet the whole fab!
+[valid] SubnetsInGW: SubnetsInGW
+
+maximum policy takes like forever ;-)
+without dependability, results almost instant
+*)
+
+abbreviation "V\<equiv>TopoS_Vertices.V"
+
+definition policy :: "vString list_graph" where
+  "policy \<equiv> \<lparr> nodesL = [V ''Statistics'',
+                        V ''SensorSink'',
+                        V ''PresenceSensor'',
+                        V ''Webcam'',
+                        V ''TempSensor'',
+                        V ''FireSensor'',
+                        V ''MissionControl1'',
+                        V ''MissionControl2'',
+                        V ''Watchdog'',
+                        V ''Bot1'',
+                        V ''Bot2'',
+                        V ''AdminPc'',
+                        V ''X1'',
+                        V ''X2'',
+                        V ''X3'',
+                        V ''X4''],
+              edgesL = [(V ''PresenceSensor'', V ''SensorSink''),
+                        (V ''Webcam'', V ''SensorSink''),
+                        (V ''TempSensor'', V ''SensorSink''),
+                        (V ''FireSensor'', V ''SensorSink''),
+                        (V ''MissionControl1'', V ''Bot1''),
+                        (V ''MissionControl1'', V ''Bot2''),
+                        (V ''MissionControl2'', V ''Bot2''),
+                        (V ''AdminPc'', V ''MissionControl2''),
+                        (V ''AdminPc'', V ''MissionControl1''),
+                        (V ''Watchdog'', V ''Bot1''),
+                        (V ''Watchdog'', V ''Bot2'')
+                        ] \<rparr>"
+
+lemma "wf_list_graph policy" by eval
+
+
+text{*Privacy for employees*}
+context begin
+  private definition "BLP_privacy_host_attributes \<equiv> [V ''Statistics'' \<mapsto> 3,
+                           V ''SensorSink'' \<mapsto> 3,
+                           V ''PresenceSensor'' \<mapsto> 2, (*less critical data*)
+                           V ''Webcam'' \<mapsto> 3
+                           ]"
+  private lemma "dom (BLP_privacy_host_attributes) \<subseteq> set (nodesL policy)"
+    by(simp add: BLP_privacy_host_attributes_def policy_def)
+  definition "BLP_privacy_m \<equiv> new_configured_list_SecurityInvariant SINVAR_LIB_BLPbasic \<lparr> 
+        node_properties = BLP_privacy_host_attributes \<rparr>"
+end
+
+
+text{*Secret corporate knowledge and intellectual property*}
+context begin
+  private definition "BLP_tradesecrets_host_attributes \<equiv> [V ''MissionControl1'' \<mapsto> 1,
+                           V ''MissionControl2'' \<mapsto> 2,
+                           V ''Bot1'' \<mapsto> 1,
+                           V ''Bot2'' \<mapsto> 2
+                           ]"
+  private lemma "dom (BLP_tradesecrets_host_attributes) \<subseteq> set (nodesL policy)"
+    by(simp add: BLP_tradesecrets_host_attributes_def policy_def)
+  definition "BLP_tradesecrets_m \<equiv> new_configured_list_SecurityInvariant SINVAR_LIB_BLPbasic \<lparr> 
+        node_properties = BLP_tradesecrets_host_attributes \<rparr>"
+end
+
+
+text{*Privacy for employees, exporting aggregated data*}
+context begin
+  private definition "BLP_employee_export_host_attributes \<equiv>
+                          [V ''Statistics'' \<mapsto> \<lparr> privacy_level = 3, trusted = False \<rparr>,
+                           V ''SensorSink'' \<mapsto> \<lparr> privacy_level = 2, trusted = True \<rparr>,
+                           V ''PresenceSensor'' \<mapsto> \<lparr> privacy_level = 2, trusted = False \<rparr>,
+                           V ''Webcam'' \<mapsto> \<lparr> privacy_level = 3, trusted = False \<rparr>
+                           ]"
+  private lemma "dom (BLP_employee_export_host_attributes) \<subseteq> set (nodesL policy)"
+    by(simp add: BLP_employee_export_host_attributes_def policy_def)
+  definition "BLP_employee_export_m \<equiv> new_configured_list_SecurityInvariant SINVAR_LIB_BLPtrusted \<lparr> 
+        node_properties = BLP_employee_export_host_attributes \<rparr>"
+end
+
+
+
+text{*Who can access bot2?*}
+context begin
+  private definition "ACL_bot2_host_attributues \<equiv>
+                          [V ''Bot2'' \<mapsto> Master [V ''Bot1'',
+                                                 V ''MissionControl1'',
+                                                 V ''MissionControl2'',
+                                                 V ''Watchdog''],
+                           V ''MissionControl1'' \<mapsto> Care,
+                           V ''MissionControl2'' \<mapsto> Care,
+                           V ''Watchdog'' \<mapsto> Care
+                           ]"
+  private lemma "dom (ACL_bot2_host_attributues) \<subseteq> set (nodesL policy)"
+    by(simp add: ACL_bot2_host_attributues_def policy_def)
+  definition "ACL_bot2_m \<equiv> new_configured_list_SecurityInvariant SINVAR_LIB_CommunicationPartners
+                             \<lparr>node_properties = ACL_bot2_host_attributues \<rparr>"
+end
+
+
+(*TODO: dependability*)
+
+
+text{*Hierarchy of fab robots*}
+context begin
+  private definition "DomainHierarchy_host_attributes \<equiv>
+                [(V ''MissionControl1'',
+                    DN (''ControlTerminal''--''ControlDevices''--Leaf, 0)),
+                 (V ''MissionControl2'',
+                    DN (''ControlTerminal''--''ControlDevices''--Leaf, 0)),
+                 (V ''Watchdog'',
+                    DN (''ControlTerminal''--''ControlDevices''--''Robots''--Leaf, 0)),
+                 (V ''Bot1'',
+                    DN (''ControlTerminal''--''ControlDevices''--''Robots''--Leaf, 0)),
+                 (V ''Bot2'',
+                    DN (''ControlTerminal''--''ControlDevices''--''Robots''--Leaf, 0)),
+                 (V ''AdminPc'',
+                    DN (''ControlTerminal''--Leaf, 0))
+                 ]"
+  private lemma "dom (map_of DomainHierarchy_host_attributes) \<subseteq> set (nodesL policy)"
+    by(simp add: DomainHierarchy_host_attributes_def policy_def)
+
+  lemma "DomainHierarchyNG_sanity_check_config
+    (map snd DomainHierarchy_host_attributes)
+        (
+        Department ''ControlTerminal'' [
+          Department ''ControlDevices'' [
+            Department ''Robots'' [],
+            Department ''OtherStuff'' [],
+            Department ''ThirdSubDomain'' []
+          ],
+          Department ''Supervision'' [
+            Department ''S1'' [],
+            Department ''S2'' []
+          ]
+        ])" by eval
+
+  definition "Control_hierarchy_m \<equiv> new_configured_list_SecurityInvariant
+                                    SINVAR_LIB_DomainHierarchyNG
+                                    \<lparr> node_properties = map_of DomainHierarchy_host_attributes \<rparr>"
+end
+
+text{*NonInterference of something (for the sake of example)
+Whatever happens, Admin must not interfere with the fire sensor.
+Because the company that sold the fire sensor wrote it in their contract or something.*}
+context begin
+  private definition "NonInterference_host_attributes \<equiv>
+                [V ''Statistics'' \<mapsto> Unrelated,
+                 V ''SensorSink'' \<mapsto> Unrelated,
+                 V ''PresenceSensor'' \<mapsto> Unrelated,
+                 V ''Webcam'' \<mapsto> Unrelated,
+                 V ''TempSensor'' \<mapsto> Unrelated,
+                 V ''FireSensor'' \<mapsto> Interfering, (*!*)
+                 V ''MissionControl1'' \<mapsto> Unrelated,
+                 V ''MissionControl2'' \<mapsto> Unrelated,
+                 V ''Watchdog'' \<mapsto> Unrelated,
+                 V ''Bot1'' \<mapsto> Unrelated,
+                 V ''Bot2'' \<mapsto> Unrelated,
+                 V ''AdminPc'' \<mapsto> Interfering, (*!*)
+                 V ''X1'' \<mapsto> Unrelated,
+                 V ''X2'' \<mapsto> Unrelated,
+                 V ''X3'' \<mapsto> Unrelated,
+                 V ''X4'' \<mapsto> Unrelated
+                 ]"
+  private lemma "dom NonInterference_host_attributes \<subseteq> set (nodesL policy)"
+    by(simp add: NonInterference_host_attributes_def policy_def)
+  definition "NonInterference_m \<equiv> new_configured_list_SecurityInvariant SINVAR_LIB_NonInterference
+                                    \<lparr> node_properties = NonInterference_host_attributes \<rparr>"
+end
+
+
+
+text{*Sensor Gateway*}
+context begin
+  private definition "SecurityGateway_host_attributes \<equiv>
+                [V ''SensorSink'' \<mapsto> SecurityGateway,
+                 V ''PresenceSensor'' \<mapsto> DomainMember,
+                 V ''Webcam'' \<mapsto> DomainMember,
+                 V ''TempSensor'' \<mapsto> DomainMember,
+                 V ''FireSensor'' \<mapsto> DomainMember
+                 ]"
+  private lemma "dom SecurityGateway_host_attributes \<subseteq> set (nodesL policy)"
+    by(simp add: SecurityGateway_host_attributes_def policy_def)
+  definition "SecurityGateway_m \<equiv> new_configured_list_SecurityInvariant
+                                  SINVAR_LIB_SecurityGatewayExtended
+                                    \<lparr> node_properties = SecurityGateway_host_attributes \<rparr>"
+end
+
+
+text{*Production Robots are an information sink*}
+context begin
+  private definition "SinkRobots_host_attributes \<equiv>
+                [V ''MissionControl1'' \<mapsto> SinkPool,
+                 V ''MissionControl2'' \<mapsto> SinkPool,
+                 V ''Bot1'' \<mapsto> Sink,
+                 V ''Bot2'' \<mapsto> Sink
+                 ]"
+  private lemma "dom SinkRobots_host_attributes \<subseteq> set (nodesL policy)"
+    by(simp add: SinkRobots_host_attributes_def policy_def)
+  definition "SinkRobots_m \<equiv> new_configured_list_SecurityInvariant
+                                  SINVAR_LIB_Sink
+                                    \<lparr> node_properties = SinkRobots_host_attributes \<rparr>"
+end
+
+text{*Subnet of the fab*}
+context begin
+  private definition "Subnets_host_attributes \<equiv>
+                [V ''Statistics'' \<mapsto> Subnet 1,
+                 V ''SensorSink'' \<mapsto> Subnet 1,
+                 V ''PresenceSensor'' \<mapsto> Subnet 1,
+                 V ''Webcam'' \<mapsto> Subnet 1,
+                 V ''TempSensor'' \<mapsto> Subnet 1,
+                 V ''FireSensor'' \<mapsto> Subnet 1,
+                 V ''AdminPc'' \<mapsto> Subnet 4,
+                 V ''X1'' \<mapsto> Subnet 8,
+                 V ''X2'' \<mapsto> Subnet 8,
+                 V ''X3'' \<mapsto> Subnet 8,
+                 V ''X4'' \<mapsto> Subnet 8
+                 ]"
+  private lemma "dom Subnets_host_attributes \<subseteq> set (nodesL policy)"
+    by(simp add: Subnets_host_attributes_def policy_def)
+  definition "Subnets_m \<equiv> new_configured_list_SecurityInvariant
+                                  SINVAR_LIB_Subnets
+                                    \<lparr> node_properties = Subnets_host_attributes \<rparr>"
+end
+
+
+context begin
+  private definition "SubnetsInGW_host_attributes \<equiv>
+                [V ''Statistics'' \<mapsto> Member,
+                 V ''SensorSink'' \<mapsto> InboundGateway
+                 ]"
+  private lemma "dom SubnetsInGW_host_attributes \<subseteq> set (nodesL policy)"
+    by(simp add: SubnetsInGW_host_attributes_def policy_def)
+  definition "SubnetsInGW_m \<equiv> new_configured_list_SecurityInvariant
+                                  SINVAR_LIB_SubnetsInGW
+                                    \<lparr> node_properties = SubnetsInGW_host_attributes \<rparr>"
+end
+
+
+definition "invariants \<equiv> [BLP_privacy_m, BLP_tradesecrets_m, BLP_employee_export_m,
+                          ACL_bot2_m, Control_hierarchy_m,
+                          SecurityGateway_m, SinkRobots_m, Subnets_m, SubnetsInGW_m]"
+ (*NonInterference_m*)
+
+(*TODO: add noninterference*)
+lemma "length invariants = 9" by eval
+
+
+(*this*)
+lemma "all_security_requirements_fulfilled invariants policy" by eval
+ML{*
+visualize_graph @{context} @{term "invariants"} @{term "policy"};
+*}
+
+
+definition make_policy :: "('a SecurityInvariant) list \<Rightarrow> 'a list \<Rightarrow> 'a list_graph" where
+  "make_policy sinvars Vs \<equiv> generate_valid_topology sinvars \<lparr>nodesL = Vs, edgesL = List.product Vs Vs \<rparr>"
+
+
+value[code] "make_policy invariants (nodesL policy)" (*15s without NonInterference*)
+
+(*TODO:*)
+(*
+value[code] "make_policy (invariants@[NonInterference_m]) (nodesL policy)"
+value[code] "make_policy (NonInterference_m#invariants) (nodesL policy)"
+*)
+
+text{*
+The diff to the maximum
+  (*?? well, there is NonInterference in it, but it should not matter here because the two parts
+   *?? of the graph are separated anyway*) policy.
+*}
+ML_val{*
+visualize_edges @{context} @{term "edgesL policy"} 
+    [("edge [dir=\"arrow\", style=dashed, color=\"#FF8822\", constraint=false]",
+     @{term "[e \<leftarrow> edgesL (make_policy invariants (nodesL policy)). e \<notin> set (edgesL policy)]"})] ""; 
+*}
+
+
+
+subsection{*stateful implementation*}
+definition "stateful_policy = generate_valid_stateful_policy_IFSACS policy invariants"
+value "stateful_policy"
+
+ML_val{*
+visualize_edges @{context} @{term "flows_fixL stateful_policy"} 
+    [("edge [dir=\"arrow\", style=dashed, color=\"#FF8822\", constraint=false]", @{term "flows_stateL stateful_policy"})] ""; 
+*}
+
+
+
+end
+
+
